mailbox/verif_atomic_exchange.v
@@ -1,18 +1,30 @@
-Require Import VST.veric.rmaps.
 Require Import VST.concurrency.conclib.
-Require Import VST.concurrency.ghosts.
-Require Import VST.floyd.library.
-Require Import VST.zlist.sublist.
-Require Import VST.concurrency.lock_specs.
-Require Import VST.atomics.verif_lock.
-Require Import mailbox.atomic_exchange.
-Require Import Lia.
-
-(* standard VST prelude *)
-#[export] Instance CompSpecs : compspecs. make_compspecs prog. Defined.
-Definition Vprog : varspecs. mk_varspecs prog. Defined.
+From iris_ora.algebra Require Import gmap frac_auth.
+Require Import VST.atomics.SC_atomics.
 
 Section AEHist.
+
+Section gmap_frac.
+
+Context K `{Countable K} (A : ofe).
+
+Lemma gmap_excl_flat : forall n (x y : gmapUR K (exclR A)), ✓{n} y → x ≼ₒ{n} y → x ≡{n}≡ y.
+Proof.
+  intros ??? Hv Hord i; specialize (Hord i).
+  hnf in Hord.
+  destruct (x !! i)%stdpp eqn: Hx, (y !! i)%stdpp eqn: Hy; rewrite Hx Hy // in Hord |- *.
+  - inv Hord; try done.
+    by repeat constructor.
+  - specialize (Hv i); rewrite Hy in Hv.
+    specialize (Hord o).
+    destruct o; try done.
+    inv Hord.
+Qed.
+
+Canonical Structure gmap_frac_authR := frac_authR gmap_excl_flat.
+Canonical Structure gmap_frac_authUR := frac_authUR gmap_excl_flat.
+
+End gmap_frac.
 
 (* These histories should be usable for any atomically accessed location. *)
 Inductive AE_hist_el := AE (r : val) (w : val).
@@ -22,8 +34,6 @@ Fixpoint apply_hist a h :=
   | [] => Some a
   | AE r w :: h' => if eq_dec r a then apply_hist w h' else None
   end.
-
-Arguments eq_dec _ _ _ _ : simpl never.
 
 Lemma apply_hist_app : forall h1 i h2, apply_hist i (h1 ++ h2) =
   match apply_hist i h1 with Some v => apply_hist v h2 | None => None end.
@@ -35,157 +45,222 @@ Qed.
 
 End AEHist.
 
-Notation hist := (nat -> option AE_hist_el).
+Notation hist := (gmap nat (excl AE_hist_el)).
+
+Fixpoint list_to_hist (l : list AE_hist_el) n : hist :=
+  match l with
+  | [] => ∅
+  | e :: rest => <[n := Excl e]> (list_to_hist rest (S n))
+  end.
+
+Lemma list_to_hist_lookup : forall l n i, (n <= i)%nat ->
+  (list_to_hist l n !! i)%stdpp = option_map Excl (nth_error l (i - n)).
+Proof.
+  induction l; simpl; intros.
+  - rewrite lookup_empty nth_error_nil //.
+  - destruct (eq_dec n i).
+    + subst; rewrite lookup_insert Nat.sub_diag //.
+    + rewrite lookup_insert_ne //.
+      destruct (i - n)%nat as [|n'] eqn: Hi; first lia.
+      rewrite IHl /=; last lia.
+      do 2 f_equal; lia.
+Qed.
+
+Lemma list_to_hist_insert : forall l n e,
+  <[(n + length l)%nat := Excl e]>(list_to_hist l n) = list_to_hist (l ++ [e]) n.
+Proof.
+  induction l; simpl; intros.
+  - rewrite Nat.add_0_r //.
+  - rewrite insert_commute; last lia.
+    replace (n + S _)%nat with (S n + length l)%nat by lia.
+    rewrite IHl //.
+Qed.
+
+Definition hist_incl (h : hist) l := forall t e, (h !! t)%stdpp = Some (Excl e) -> nth_error l t = Some e.
+
+Definition newer (l : hist) t := forall t', (l !! t')%stdpp <> None -> (t' < t)%nat.
+
+Lemma hist_incl_lt : forall (h : hist) l (Hv : ✓ (h : gmapUR _ (exclR (leibnizO _)))),
+  hist_incl h l -> newer h (length l).
+Proof.
+  unfold hist_incl; repeat intro.
+  specialize (H t'); specialize (Hv t').
+  destruct (h !! t')%stdpp as [e|] eqn: Ht'; [|contradiction].
+  rewrite Ht' in Hv.
+  destruct e; try done.
+  by apply nth_error_Some; erewrite H.
+Qed.
+
+Section AE.
+
+Context `{!VSTGS OK_ty Σ} `{!inG Σ (gmap_frac_authR nat (leibnizO AE_hist_el))}
+  `{!atomic_int_impl}.
+
+Definition ghost_ref h g := own g (●F (list_to_hist h O : gmapR _ (exclR (leibnizO _)))).
+Definition ghost_hist q (h : gmap nat (excl AE_hist_el)) g := own g (◯F{q} (h : gmapR _ (exclR (leibnizO _)))).
+
+Lemma hist_ref_incl : forall sh h h' p,
+  ghost_hist sh h p ∗ ghost_ref h' p ⊢ ⌜hist_incl h h'⌝.
+Proof.
+  intros; iIntros "(Hh & Hr)".
+  iPoseProof (own_valid_2 with "Hr Hh") as "H".
+  rewrite frac_auth_agreeI.
+  if_tac.
+  - iDestruct "H" as "(%Hh & _)"; iPureIntro.
+    apply leibniz_equiv in Hh as <-.
+    intros ??.
+    rewrite list_to_hist_lookup; last lia.
+    destruct (nth_error _ _) eqn: E; inversion 1; subst.
+    rewrite Nat.sub_0_r // in E.
+  - iDestruct "H" as "(%Hh & _)"; iPureIntro.
+    assert (forall i, cmra.included(A := cmra.optionR (iris.algebra.excl.exclR (leibnizO AE_hist_el)))
+      (h !! i)%stdpp (list_to_hist h' 0 !! i)%stdpp) as Hincl.
+    { rewrite -gmap.lookup_included //. }
+    intros ?? Ht.
+    specialize (Hincl t); rewrite Ht list_to_hist_lookup in Hincl; last lia.
+    rewrite  Nat.sub_0_r in Hincl.
+    destruct (nth_error h' t) eqn: Hnth.
+    rewrite Excl_included in Hincl; rewrite Hincl //.
+    { rewrite option_included in Hincl.
+      destruct Hincl as [| (? & ? & ? & ? & ?)]; done. }
+Qed.
+
+Lemma hist_add' : forall sh h h' e p,
+  ghost_hist sh h p ∗ ghost_ref h' p ⊢ |==>
+  ghost_hist sh (<[length h' := Excl e]>h) p ∗ ghost_ref (h' ++ [e]) p.
+Proof.
+  intros; iIntros "(Hh & Hr)".
+  iMod (own_update_2 with "Hr Hh") as "H".
+  { apply (@frac_auth_update (iris.algebra.gmap.gmapR _ _) sh (list_to_hist h' 0:
+      iris.algebra.gmap.gmapUR nat (iris.algebra.excl.exclR (leibnizO AE_hist_el)))).
+    apply (gmap.alloc_local_update _ _ (length h') ((Excl e) : exclR (leibnizO _))); last done.
+    rewrite list_to_hist_lookup; last lia.
+    rewrite (proj2 (nth_error_None _ _)) //; lia. }
+  iDestruct (own_op with "H") as "(Hr & $)".
+  rewrite (list_to_hist_insert _ O) //.
+Qed.
 
 (* the lock invariant used to encode an atomic invariant *)
-Definition AE_inv x g i R := EX h : list AE_hist_el, EX v : val,
-  !!(apply_hist i h = Some v /\ tc_val tint v) &&
-  (data_at Ews tint v x * ghost_ref h g * R h v).
+Definition AE_inv x g i (R : list AE_hist_el -d> val -d> mpred) := ∃ h v, ⌜apply_hist i h = Some v /\ tc_val tint v⌝ ∧
+  (atomic_int_at Ews v x ∗ ghost_ref h g ∗ R h v).
+
+#[export] Instance AE_inv_ne x g i : NonExpansive (AE_inv x g i).
+Proof. solve_proper. Qed.
 
 Lemma AE_inv_exclusive : forall x g i R, exclusive_mpred (AE_inv x g i R).
 Proof.
   unfold AE_inv; intros.
-  eapply derives_exclusive, exclusive_sepcon1 with (Q := EX h : list AE_hist_el, EX v : val, _),
-    data_at__exclusive with (sh := Ews)(t := tint); auto; simpl; try lia.
-  Intros h v; rewrite sepcon_assoc; apply sepcon_derives; [cancel|].
-  Exists h v; apply derives_refl.
-Qed.
-#[export] Hint Resolve AE_inv_exclusive : core.
-
-Definition AE_loc sh l p g i R (h : hist) := lock_inv sh l (AE_inv p g i R) * ghost_hist sh h g.
-
-Lemma AE_inv_super_non_expansive : forall n p g i R,
-  compcert_rmaps.RML.R.approx n (AE_inv p g i R) =
-  compcert_rmaps.RML.R.approx n (AE_inv p g i (fun h v => compcert_rmaps.RML.R.approx n (R h v))).
-Proof.
-  intros; unfold AE_inv.
-  rewrite !approx_exp; apply f_equal; extensionality h.
-  rewrite !approx_exp; apply f_equal; extensionality v.
-  rewrite !approx_andp, !approx_sepcon.
-  rewrite approx_idem; auto.
+  rewrite /exclusive_mpred; iIntros "((% & % & % & Ha & _) & (% & % & % & Hb & _))".
+  iApply atomic_int_conflict; last iFrame; auto.
 Qed.
 
-Lemma AE_loc_super_non_expansive : forall n sh l p g i R h,
-  compcert_rmaps.RML.R.approx n (AE_loc sh l p g i R h) =
-  compcert_rmaps.RML.R.approx n (AE_loc sh l p g i (fun h v => compcert_rmaps.RML.R.approx n (R h v)) h).
-Proof.
-  intros; unfold AE_loc.
-  rewrite !approx_sepcon; f_equal.
-  setoid_rewrite lock_inv_super_non_expansive; do 2 f_equal.
-  rewrite AE_inv_super_non_expansive; auto.
-Qed.
+Definition AE_loc sh p g i (R : list AE_hist_el -d> val -d> mpred) (h : hist) := inv (nroot .@ "AE") (AE_inv p g i R) ∗ ghost_hist sh h g.
+
+#[export] Instance AE_loc_ne sh p g i n : Proper (dist n ==> eq ==> dist n) (AE_loc sh p g i).
+Proof. solve_proper. Qed.
 
 (* This predicate describes the valid pre- and postconditions for a given atomic invariant R. *)
-Definition AE_spec i P R Q := ALL hc : _, ALL hx : _, ALL vc : _, ALL vx : _,
-  !!(apply_hist i hx = Some vx /\ hist_incl hc hx) -->
-  ((R hx vx * P hc vc) -* (|==> R (hx ++ [AE vx vc]) vc *
-    Q (map_upd hc (length hx) (AE vx vc)) vx)).
+Definition AE_spec i (P : hist -d> val -d> mpred) (R : list AE_hist_el -d> val -d> mpred) (Q : hist -d> val -d> mpred) := ∀ hc hx vc vx,
+  ⌜apply_hist i hx = Some vx /\ hist_incl hc hx⌝ →
+  ((▷R hx vx ∗ P hc vc) -∗ (|==> ▷R (hx ++ [AE vx vc]) vc ∗
+    Q (<[length hx := Excl (AE vx vc)]>hc) vx)).
 
-Lemma AE_spec_super_non_expansive : forall n i P R Q, compcert_rmaps.RML.R.approx n (AE_spec i P R Q) =
-  compcert_rmaps.RML.R.approx n (AE_spec i (fun h v => compcert_rmaps.RML.R.approx n (P h v))
-                                           (fun h v => compcert_rmaps.RML.R.approx n (R h v))
-                                           (fun h v => compcert_rmaps.RML.R.approx n (Q h v))).
-Proof.
-  intros; unfold AE_spec.
-  rewrite !(approx_allp _ _ _ empty_map); apply f_equal; extensionality.
-  rewrite !(approx_allp _ _ _ []); apply f_equal; extensionality.
-  rewrite !(approx_allp _ _ _ Vundef); apply f_equal; extensionality.
-  rewrite !(approx_allp _ _ _ Vundef); apply f_equal; extensionality.
-  setoid_rewrite approx_imp; f_equal; f_equal.
-  rewrite view_shift_nonexpansive, !approx_sepcon; auto.
-Qed.
+#[export] Instance AE_spec_ne i : NonExpansive3 (AE_spec i).
+Proof. solve_proper. Qed.
 
 Definition AE_type := ProdType (ProdType (ProdType
-  (ConstType (share * val * gname * lock_handle * val * val * hist))
-  (ArrowType (ConstType hist) (ArrowType (ConstType val) Mpred)))
-  (ArrowType (ConstType (list AE_hist_el)) (ArrowType (ConstType val) Mpred)))
-  (ArrowType (ConstType hist) (ArrowType (ConstType val) Mpred)).
+  (ConstType (Qp * val * gname * val * val * hist))
+  (DiscreteFunType hist (DiscreteFunType val Mpred)))
+  (DiscreteFunType (list AE_hist_el) (DiscreteFunType val Mpred)))
+  (DiscreteFunType hist (DiscreteFunType val Mpred)).
 
 (* specification of atomic exchange *)
-Program Definition atomic_exchange_spec := DECLARE _simulate_atomic_exchange
-  TYPE AE_type WITH lsh : share, tgt : val, g : gname, l : lock_handle,
+Program Definition atomic_exchange_spec :=
+  TYPE AE_type WITH lsh : Qp, tgt : val, g : gname,
     i : val, v : val, h : hist, P : hist -> val -> mpred, R : list AE_hist_el -> val -> mpred, Q : hist -> val -> mpred
-  PRE [ tptr tint, tptr t_lock, tint ]
-   PROP (tc_val tint v; readable_share lsh)
-   PARAMS (tgt; ptr_of l; v) GLOBALS ()
-   SEP (AE_loc lsh l tgt g i R h; P h v; AE_spec i P R Q)
+  PRE [ tptr tint, tint ]
+   PROP (tc_val tint v)
+   PARAMS (tgt;  v) GLOBALS ()
+   SEP (AE_loc lsh tgt g i R h; P h v; AE_spec i P R Q)
   POST [ tint ]
-   EX t : nat, EX v' : val,
+   ∃ t : nat, ∃ v' : val,
    PROP (tc_val tint v'; newer h t)
    LOCAL (temp ret_temp v')
-   SEP (AE_loc lsh l tgt g i R (map_upd h t (AE v' v)); Q (map_upd h t (AE v' v)) v').
+   SEP (AE_loc lsh tgt g i R (<[t := Excl (AE v' v)]>h); Q (<[t := Excl (AE v' v)]>h) v').
 Next Obligation.
 Proof.
-  repeat intro.
-  destruct x as (((((((((?, ?), ?), ?), ?), ?), ?), P), R), Q); simpl.
-  unfold PROPx, PARAMSx, GLOBALSx, LOCALx, SEPx, argsassert2assert; simpl; rewrite !approx_andp; f_equal; f_equal;
-    rewrite !sepcon_emp, ?approx_sepcon, ?approx_idem.
-  rewrite AE_loc_super_non_expansive; do 3 f_equal.
-  apply AE_spec_super_non_expansive.
+  intros ? ((((((((?, ?), ?), ?), ?), ?), ?), ?), ?) (((((?, ?), ?), ?), ?), ?) ((([=] & ?) & ?) & ?) rho; simpl in *; subst; simpl in *.
+  solve_proper.
 Qed.
 Next Obligation.
 Proof.
-  repeat intro.
-  destruct x as (((((((((?, ?), ?), ?), ?), ?), ?), P), R), Q); simpl.
-  rewrite !approx_exp; apply f_equal; extensionality t.
-  rewrite !approx_exp; apply f_equal; extensionality v'.
-  unfold PROPx, LOCALx, SEPx; simpl; rewrite !approx_andp; f_equal; f_equal;
-    rewrite !sepcon_emp, ?approx_sepcon, ?approx_idem, AE_loc_super_non_expansive; auto.
+  intros ? ((((((((?, ?), ?), ?), ?), ?), ?), ?), ?) (((((?, ?), ?), ?), ?), ?) ((([=] & ?) & ?) & ?) rho; simpl in *; subst; simpl in *.
+  solve_proper.
 Qed.
 
-Definition Gprog : funspecs := ltac:(with_library prog [acquire_spec; release_spec; atomic_exchange_spec]).
+(* to SC_atomics? *)
+Axiom atomic_int_timeless : forall sh v p, Timeless (atomic_int_at sh v p).
+#[export] Existing Instance atomic_int_timeless.
 
-(* proof of the lock-based implementation of atomic exchange *)
-Lemma body_atomic_exchange : semax_body Vprog Gprog f_simulate_atomic_exchange atomic_exchange_spec.
-Proof. 
-  start_dep_function.
-  unfold AE_loc; Intros.
-  forward_call (lsh, l, AE_inv tgt g i R).
-  unfold AE_inv at 2; Intros h' v'.
-  assert (lsh <> Share.bot).
-  { intro; subst; contradiction unreadable_bot. }
-  forward.
-  forward.
-  assert (apply_hist i (h' ++ [AE v' v]) = Some v) as Hh'.
-  { rewrite apply_hist_app.
-    replace (apply_hist i h') with (Some v'); simpl.
-    apply eq_dec_refl. }
-  gather_SEP (ghost_hist _ _ _) (ghost_ref _ _).
-  assert_PROP (hist_incl h h') as Hincl.
-  { go_lower; apply sepcon_derives_prop.
-    rewrite hist_ref_join by auto.
-    Intros hr.
-    apply prop_right; eapply hist_sub_list_incl; eauto. }
-  viewshift_SEP 0
-    (ghost_hist lsh (map_upd h (length h') (AE v' v)) g * ghost_ref (h' ++ [AE v' v]) g)
-    by (go_lower; eapply derives_trans, bupd_fupd; apply hist_add').
-  gather_SEP (AE_spec _ _ _ _) (R h' v') (P h v); rewrite sepcon_assoc; simpl.
-  viewshift_SEP 0 (R (h' ++ [AE v' v]) v * Q (map_upd h (length h') (AE v' v)) v').
-  { go_lower; unfold AE_spec.
-    eapply derives_trans, bupd_fupd.
-    eapply derives_trans; [apply allp_sepcon1 | apply allp_left with h].
-    eapply derives_trans; [apply allp_sepcon1 | apply allp_left with h'].
-    eapply derives_trans; [apply allp_sepcon1 | apply allp_left with (Vint v)].
-    eapply derives_trans; [apply allp_sepcon1 | apply allp_left with (Vint v')].
-    rewrite prop_imp by auto.
-    rewrite sepcon_comm; apply modus_ponens_wand. }
-  forward_call release_simple (lsh, l, AE_inv tgt g i R).
-  { lock_props.
-    unfold AE_inv.
-    Exists (h' ++ [AE v' v]) v; entailer!; cancel.
-  }
-  forward.
-  Exists (length h') (Vint v'). unfold AE_loc; entailer!.
-  apply hist_incl_lt; auto.
-Qed.
-
-Lemma AE_loc_join : forall sh1 sh2 sh l p g i R h1 h2 (Hjoin : sepalg.join sh1 sh2 sh)
-  (Hsh1 : readable_share sh1) (Hsh2 : readable_share sh2) (Hcompat : disjoint h1 h2),
-  AE_loc sh1 l p g i R h1 * AE_loc sh2 l p g i R h2 = AE_loc sh l p g i R (map_add h1 h2).
+Lemma AE_sub : funspec_sub SC_atomics.atomic_exchange_spec atomic_exchange_spec.
 Proof.
-  intros; unfold AE_loc.
-  match goal with |- (?P1 * ?Q1) * (?P2 * ?Q2) = _ => transitivity ((P1 * P2) * (Q1 * Q2));
-    [apply pred_ext; cancel|] end.
-  erewrite lock_inv_share_join, ghost_hist_join by (eauto; intro; subst; contradiction unreadable_bot).
-  rewrite prop_true_andp; auto.
+  split; first done.
+  intros ((((((((q, p), g), i), v), h), P), R), Q) ?; simpl.
+  iIntros "(% & (% & _) & % & H) !>"; iExists (p, v, ⊤, ∅,
+    fun v' => ∃ t, ⌜tc_val tint v' /\ newer h t⌝ ∧ AE_loc q p g i R (<[t := Excl (AE v' v)]>h) ∗ Q (<[t := Excl (AE v' v)]>h) v'), emp.
+  iSplit.
+  - repeat (iSplit; first done).
+    rewrite /SEPx /= /LOCALx /argsassert2assert /=; monPred.unseal.
+    repeat (iSplit; first done).
+    iDestruct "H" as "(_ & (#I & hist) & P & spec & _)".
+    iSplit; last done.
+    iInv "I" as "(% & % & HI)" "Hclose".
+    rewrite bi.later_and; iDestruct "HI" as "(>(%Hh0 & %) & >Hp & >ref & R)".
+    iApply fupd_mask_intro; first set_solver; iIntros "Hmask".
+    iExists _, _; iFrame "Hp"; iSplit; first done.
+    iIntros "Hp".
+    iMod "Hmask" as "_".
+    iDestruct (own_valid with "hist") as "#Hh".
+    rewrite frac_auth_frag_validI ouPred.discrete_valid.
+    iDestruct "Hh" as "(_ & %)".
+    iDestruct (hist_ref_incl with "[$hist $ref]") as %?.
+    iMod (hist_add' with "[$hist $ref]") as "(hist & ref)".
+    rewrite /AE_spec.
+    iMod ("spec" with "[%] [$P $R]") as "(R & Q)"; first done.
+    iMod ("Hclose" with "[Hp ref R]") as "_".
+    { rewrite /AE_inv; iNext.
+      iExists _, _; iFrame; iPureIntro.
+      repeat (split; auto).
+      rewrite apply_hist_app Hh0 /=.
+      apply eq_dec_refl. }
+    iIntros "!>"; iExists _; iFrame.
+    iSplit; last done.
+    iPureIntro; split; auto.
+    apply hist_incl_lt; done.
+  - iPureIntro; intros.
+    iIntros "(% & _ & % & _ & ? & H & _)"; simpl.
+    iDestruct "H" as (t ?) "(? & ?)".
+    iExists t, v'; iSplit.
+    { simpl; iPureIntro; tauto. }
+    iSplit; first done.
+    simpl; iFrame.
 Qed.
+
+Search Op gmap.
+
+Lemma AE_loc_join : forall sh1 sh2 p g i R h1 h2,
+  AE_loc sh1 p g i R h1 ∗ AE_loc sh2 p g i R h2 ⊣⊢ AE_loc (sh1 ⋅ sh2) p g i R (@op _ (gmap.gmap_op_instance(A := exclR (leibnizO _))) h1 h2).
+Proof.
+  intros; rewrite /AE_loc.
+  assert (ghost_hist (sh1 ⋅ sh2) (h1 ⋅ h2) g ⊣⊢ ghost_hist sh1 h1 g ∗ ghost_hist sh2 h2 g) as ->.
+  { rewrite -own_op. rewrite /ghost_hist; f_equiv.
+    rewrite frac_op.
+    apply (@frac_auth_frag_op (gmapR _ (exclR (leibnizO _))) sh1 sh2 h1 h2). }
+  iSplit.
+  - iIntros "(($ & $) & (_ & $))".
+  - iIntros "(#$ & $ & $)".
+Qed.
+
+End AE.
+
+#[export] Hint Resolve AE_inv_exclusive : core.
